WIP: outline of the new finiteness lemma for fairness

fairness/fairness_finiteness.v
@@ -19,6 +19,11 @@ Section gmap.
   Qed.
 End gmap.
 
+(* TODO: unify with [rel_finitary] which requires a Trillium model and does not use Finite *)
+Definition rel_finitary' {Λ St Lb} ξ :=
+  ∀ (ex : execution_trace Λ) (atr : finite_trace St Lb) c' oζ,
+    smaller_card (sig (λ '(δ', ℓ), ξ (ex :tr[oζ]: c') (atr :tr[ℓ]: δ'))) nat.
+
 Section finitary.
   Context `{M: FairModel}.
   Context `{Λ: language}.
@@ -28,21 +33,56 @@ Section finitary.
 
   Context `{HPI0: forall s x, ProofIrrel ((let '(s', ℓ) := x in M.(fmtrans) s ℓ s'): Prop) }.
 
-  Variable model_finitary: forall s1, Finite { '(s2, ℓ) | M.(fmtrans) s1 ℓ s2 }.
+  Variable (ξ: execution_trace Λ -> finite_trace M (option M.(fmrole)) -> Prop).
 
-  Definition enum_inner (s1: M): list (M * option M.(fmrole)) :=
-    map proj1_sig (@enum _ _ (model_finitary s1)).
+  Variable model_finitary: rel_finitary' ξ.
 
-  Lemma enum_inner_spec (s1 s2: M) ℓ:
-    M.(fmtrans) s1 ℓ s2 -> (s2, ℓ) ∈ enum_inner s1.
-  Proof.
-    intros H. unfold enum_inner. rewrite elem_of_list_fmap.
-    exists (exist _ (s2, ℓ) H). split =>//. apply elem_of_enum.
-  Qed.
+  #[local] Instance eq_dec_next_states ex atr c' oζ:
+    EqDecision {'(δ', ℓ) : M * (option (fmrole M)) |
+                  ξ (ex :tr[ oζ ]: c') (atr :tr[ ℓ ]: δ')}.
+  Proof. Admitted.
 
-  Program Definition enumerate_next (δ1: LM) (oζ : olocale Λ) (c': cfg Λ):
+  Lemma model_finite: ∀ (ex : execution_trace Λ) (atr : finite_trace _ _) c' oζ,
+    Finite (sig (λ '(δ', ℓ), ξ (ex :tr[oζ]: c') (atr :tr[ℓ]: δ'))).
+  Proof. Admitted.
+
+  Definition enum_inner extr fmodtr c' oζ: list (M * option M.(fmrole)) :=
+    map proj1_sig (@enum _ _ (model_finite extr fmodtr c' oζ)).
+
+  (* Lemma enum_inner_spec (s1 s2: M) ℓ extr fmodtr c' oζ: *)
+  (*   M.(fmtrans) s1 ℓ s2 -> (s2, ℓ) ∈ enum_inner extr fmodtr c' oζ. *)
+  (* Proof. *)
+  (*   intros H. unfold enum_inner. rewrite elem_of_list_fmap. *)
+  (*   exists (exist _ (s2, ℓ) H). split =>//. apply elem_of_enum. *)
+  (* Qed. *)
+
+  (* TODO: move *)
+  Fixpoint trace_map {A A' L L'} (sf: A → A') (lf: L -> L') (tr: finite_trace A L): finite_trace A' L' :=
+  match tr with
+  | trace_singleton x => trace_singleton $ sf x
+  | trace_extend tr' ℓ x => trace_extend (trace_map sf lf tr') (lf ℓ) (sf x)
+  end.
+
+  Fixpoint get_underlying_fairness_trace (M : FairModel) (LM: LiveModel Λ M) (ex : auxiliary_trace LM) :=
+  match ex with
+  | trace_singleton δ => trace_singleton (ls_under δ)
+  | trace_extend ex' (Take_step ρ _) δ => trace_extend (get_underlying_fairness_trace M LM ex') ρ (ls_under δ)
+  | trace_extend ex' _ _ => get_underlying_fairness_trace M LM ex'
+  end.
+
+  Definition get_role {M : FairModel} {LM: LiveModel Λ M} (lab: mlabel LM) :=
+  match lab with
+  | Take_step ρ _ => Some ρ
+  | _ => None
+  end.
+
+  Definition map_underlying_trace {M : FairModel} {LM: LiveModel Λ M} (aux : auxiliary_trace LM) :=
+    (trace_map (λ s, ls_under s) (λ lab, get_role lab) aux).
+
+  Program Definition enumerate_next extr (fmodtr: auxiliary_trace LM) c' oζ:
     list (LM * @mlabel LM) :=
-    '(s2, ℓ) ← (δ1.(ls_under), None) :: enum_inner δ1.(ls_under);
+    let δ1 := trace_last fmodtr in
+    '(s2, ℓ) ← (δ1.(ls_under), None) :: enum_inner extr (map_underlying_trace fmodtr) c' oζ;
     d ← enumerate_dom_gsets' (dom δ1.(ls_fuel) ∪ live_roles _ s2);
     fs ← enum_gmap_bounded' (live_roles _ s2 ∪ d) (max_gmap δ1.(ls_fuel) `max` LM.(fuel_limit) s2);
     ms ← enum_gmap_range_bounded' (live_roles _ s2 ∪ d) (locales_of_list c'.1);
@@ -70,80 +110,97 @@ Section finitary.
   Qed.
 
   Lemma valid_state_evolution_finitary_fairness (φ: execution_trace Λ -> auxiliary_trace LM -> Prop) :
-    rel_finitary (valid_lift_fairness φ).
+    rel_finitary (valid_lift_fairness (λ extr auxtr, ξ extr (map_underlying_trace auxtr) ∧ φ extr auxtr)).
   Proof.
-    intros extr auxtr [e' σ'] oζ.
-    eapply finite_smaller_card_nat.
-    eapply (in_list_finite (enumerate_next (trace_last auxtr) oζ (e',σ'))).
-    intros [δ2 ℓ] [[Hlab [Htrans Hsmall]] ?].
-    unfold enumerate_next. apply elem_of_list_bind.
-    exists (δ2.(ls_under), match ℓ with Take_step l _ => Some l | _ => None end).
-    split; last first.
-    { destruct ℓ as [ρ tid' | |].
-      - inversion Htrans as [Htrans']. apply elem_of_cons; right. by apply enum_inner_spec.
-      - apply elem_of_cons; left. f_equal. inversion Htrans as (?&?&?&?&?); done.
-      - apply elem_of_cons; right. inversion Htrans as (?&?). by apply enum_inner_spec. }
-    apply elem_of_list_bind. eexists (dom $ δ2.(ls_fuel)). split; last first.
-    { apply enumerate_dom_gsets'_spec. destruct ℓ as [ρ tid' | |].
-      - inversion Htrans as (?&?&?&?&?&?&?). intros ρ' Hin. destruct (decide (ρ' ∈ live_roles _ δ2)); first set_solver.
-        destruct (decide (ρ' ∈ dom $ ls_fuel (trace_last auxtr))); first set_solver. set_solver.
-      - inversion Htrans as (?&?&?&?&?). set_solver.
-      - inversion Htrans as (?&?&?&?&?). done. }
-    apply elem_of_list_bind.
-    assert (Hfueldom: dom δ2.(ls_fuel) = live_roles M δ2 ∪ dom (ls_fuel δ2)).
-    { rewrite subseteq_union_1_L //. apply ls_fuel_dom. }
+    (* intros extr auxtr [e' σ'] oζ. *)
+    (* eapply finite_smaller_card_nat. *)
+    (* eapply (in_list_finite (enumerate_next (trace_last auxtr) oζ (e',σ'))). *)
+    (* intros [δ2 ℓ] [[Hlab [Htrans Hsmall]] ?]. *)
+    (* unfold enumerate_next. apply elem_of_list_bind. *)
+    (* exists (δ2.(ls_under), match ℓ with Take_step l _ => Some l | _ => None end). *)
+    (* split; last first. *)
+    (* { destruct ℓ as [ρ tid' | |]. *)
+    (*   - inversion Htrans as [Htrans']. apply elem_of_cons; right. by apply enum_inner_spec. *)
+    (*   - apply elem_of_cons; left. f_equal. inversion Htrans as (?&?&?&?&?); done. *)
+    (*   - apply elem_of_cons; right. inversion Htrans as (?&?). by apply enum_inner_spec. } *)
+    (* apply elem_of_list_bind. eexists (dom $ δ2.(ls_fuel)). split; last first. *)
+    (* { apply enumerate_dom_gsets'_spec. destruct ℓ as [ρ tid' | |]. *)
+    (*   - inversion Htrans as (?&?&?&?&?&?&?). intros ρ' Hin. destruct (decide (ρ' ∈ live_roles _ δ2)); first set_solver. *)
+    (*     destruct (decide (ρ' ∈ dom $ ls_fuel (trace_last auxtr))); first set_solver. set_solver. *)
+    (*   - inversion Htrans as (?&?&?&?&?). set_solver. *)
+    (*   - inversion Htrans as (?&?&?&?&?). done. } *)
+    (* apply elem_of_list_bind. *)
+    (* assert (Hfueldom: dom δ2.(ls_fuel) = live_roles M δ2 ∪ dom (ls_fuel δ2)). *)
+    (* { rewrite subseteq_union_1_L //. apply ls_fuel_dom. } *)
 
-    eexists (δ2.(ls_fuel) ↾ Hfueldom); split; last first.
-    { eapply enum_gmap_bounded'_spec; split =>//.
-      intros ρ f Hsome. destruct ℓ as [ρ' tid' | |].
-      - destruct (decide (ρ = ρ')) as [-> | Hneq].
-        + inversion Htrans as [? Hbig]. destruct Hbig as (Hmap&Hleq&?&Hlim&?&?).
-          destruct (decide (ρ' ∈ live_roles _ δ2)).
-          * rewrite Hsome /= in Hlim.
-            assert (Hlive: ρ' ∈ live_roles _ δ2) by set_solver.
-            specialize (Hlim Hlive). lia.
-          * unfold fuel_decr in Hleq.
-            apply elem_of_dom_2 in Hmap. rewrite ls_same_doms in Hmap.
-            pose proof Hsome as Hsome'. apply elem_of_dom_2 in Hsome'.
-            specialize (Hleq ρ' ltac:(done) ltac:(done)).
-            assert(must_decrease ρ' (Some ρ') (trace_last auxtr) δ2 (Some tid')) as Hmd; first by constructor 3.
-            specialize (Hleq Hmd). rewrite Hsome /= in Hleq.
-            apply elem_of_dom in Hmap as [? Heq]. rewrite Heq in Hleq.
-            pose proof (max_gmap_spec _ _ _ Heq). simpl in *. lia.
-        + inversion Htrans as [? Hbig]. destruct Hbig as (Hmap&?&Hleq'&?&Hnew&?).
-          destruct (decide (ρ ∈ dom $ ls_fuel (trace_last auxtr))) as [Hin|Hnotin].
-          * assert (Hok: oleq (ls_fuel δ2 !! ρ) (ls_fuel (trace_last auxtr) !! ρ)).
-            { unfold fuel_must_not_incr in *.
-              assert (ρ ∈ dom $ ls_fuel (trace_last auxtr)) by SS.
-              specialize (Hleq' ρ ltac:(done) ltac:(congruence)) as [Hleq'|Hleq'] =>//. apply elem_of_dom_2 in Hsome. set_solver. }
-            rewrite Hsome in Hok. destruct (ls_fuel (trace_last auxtr) !! ρ) as [f'|] eqn:Heqn; last done.
-            pose proof (max_gmap_spec _ _ _ Heqn). simpl in *. lia.
-          * assert (Hok: oleq (ls_fuel δ2 !! ρ) (Some (LM.(fuel_limit) δ2))).
-            { apply Hnew. apply elem_of_dom_2 in Hsome. set_solver. }
-            rewrite Hsome in Hok. simpl in Hok. lia.
-      - inversion Htrans as [? [? [Hleq [Hincl Heq]]]]. specialize (Hleq ρ).
-        assert (ρ ∈ dom $ ls_fuel (trace_last auxtr)) as Hin.
-        { apply elem_of_dom_2 in Hsome. set_solver. }
-        specialize (Hleq Hin ltac:(done)) as [Hleq|Hleq].
-        + rewrite Hsome in Hleq. destruct (ls_fuel (trace_last auxtr) !! ρ) as [f'|] eqn:Heqn; last done.
-          pose proof (max_gmap_spec _ _ _ Heqn). simpl in *. lia.
-        + apply elem_of_dom_2 in Hsome. set_solver.
-      - inversion Htrans as [? [? [Hleq [Hnew Hfalse]]]]. done. }
-    apply elem_of_list_bind.
-    assert (Hmappingdom: dom δ2.(ls_mapping) = live_roles M δ2 ∪ dom (ls_fuel δ2)).
-    { rewrite -Hfueldom ls_same_doms //. }
+    (* eexists (δ2.(ls_fuel) ↾ Hfueldom); split; last first. *)
+    (* { eapply enum_gmap_bounded'_spec; split =>//. *)
+    (*   intros ρ f Hsome. destruct ℓ as [ρ' tid' | |]. *)
+    (*   - destruct (decide (ρ = ρ')) as [-> | Hneq]. *)
+    (*     + inversion Htrans as [? Hbig]. destruct Hbig as (Hmap&Hleq&?&Hlim&?&?). *)
+    (*       destruct (decide (ρ' ∈ live_roles _ δ2)). *)
+    (*       * rewrite Hsome /= in Hlim. *)
+    (*         assert (Hlive: ρ' ∈ live_roles _ δ2) by set_solver. *)
+    (*         specialize (Hlim Hlive). lia. *)
+    (*       * unfold fuel_decr in Hleq. *)
+    (*         apply elem_of_dom_2 in Hmap. rewrite ls_same_doms in Hmap. *)
+    (*         pose proof Hsome as Hsome'. apply elem_of_dom_2 in Hsome'. *)
+    (*         specialize (Hleq ρ' ltac:(done) ltac:(done)). *)
+    (*         assert(must_decrease ρ' (Some ρ') (trace_last auxtr) δ2 (Some tid')) as Hmd; first by constructor 3. *)
+    (*         specialize (Hleq Hmd). rewrite Hsome /= in Hleq. *)
+    (*         apply elem_of_dom in Hmap as [? Heq]. rewrite Heq in Hleq. *)
+    (*         pose proof (max_gmap_spec _ _ _ Heq). simpl in *. lia. *)
+    (*     + inversion Htrans as [? Hbig]. destruct Hbig as (Hmap&?&Hleq'&?&Hnew&?). *)
+    (*       destruct (decide (ρ ∈ dom $ ls_fuel (trace_last auxtr))) as [Hin|Hnotin]. *)
+    (*       * assert (Hok: oleq (ls_fuel δ2 !! ρ) (ls_fuel (trace_last auxtr) !! ρ)). *)
+    (*         { unfold fuel_must_not_incr in *. *)
+    (*           assert (ρ ∈ dom $ ls_fuel (trace_last auxtr)) by SS. *)
+    (*           specialize (Hleq' ρ ltac:(done) ltac:(congruence)) as [Hleq'|Hleq'] =>//. apply elem_of_dom_2 in Hsome. set_solver. } *)
+    (*         rewrite Hsome in Hok. destruct (ls_fuel (trace_last auxtr) !! ρ) as [f'|] eqn:Heqn; last done. *)
+    (*         pose proof (max_gmap_spec _ _ _ Heqn). simpl in *. lia. *)
+    (*       * assert (Hok: oleq (ls_fuel δ2 !! ρ) (Some (LM.(fuel_limit) δ2))). *)
+    (*         { apply Hnew. apply elem_of_dom_2 in Hsome. set_solver. } *)
+    (*         rewrite Hsome in Hok. simpl in Hok. lia. *)
+    (*   - inversion Htrans as [? [? [Hleq [Hincl Heq]]]]. specialize (Hleq ρ). *)
+    (*     assert (ρ ∈ dom $ ls_fuel (trace_last auxtr)) as Hin. *)
+    (*     { apply elem_of_dom_2 in Hsome. set_solver. } *)
+    (*     specialize (Hleq Hin ltac:(done)) as [Hleq|Hleq]. *)
+    (*     + rewrite Hsome in Hleq. destruct (ls_fuel (trace_last auxtr) !! ρ) as [f'|] eqn:Heqn; last done. *)
+    (*       pose proof (max_gmap_spec _ _ _ Heqn). simpl in *. lia. *)
+    (*     + apply elem_of_dom_2 in Hsome. set_solver. *)
+    (*   - inversion Htrans as [? [? [Hleq [Hnew Hfalse]]]]. done. } *)
+    (* apply elem_of_list_bind. *)
+    (* assert (Hmappingdom: dom δ2.(ls_mapping) = live_roles M δ2 ∪ dom (ls_fuel δ2)). *)
+    (* { rewrite -Hfueldom ls_same_doms //. } *)
 
-    exists (δ2.(ls_mapping) ↾ Hmappingdom); split; last first.
-    { eapply enum_gmap_range_bounded'_spec; split=>//.
-      intros ρ' tid' Hsome. unfold tids_smaller in *.
-      apply locales_of_list_from_locale_from. eauto. }
-    rewrite elem_of_list_singleton; f_equal.
-    - destruct δ2; simpl. f_equal; apply ProofIrrelevance.
-    - destruct ℓ; simpl; destruct oζ =>//; by inversion Hlab.
-      Unshelve.
-      + intros ??. apply make_decision.
-      + intros. apply make_proof_irrel.
-      + done.
-      + done.
-  Qed.
+    (* exists (δ2.(ls_mapping) ↾ Hmappingdom); split; last first. *)
+    (* { eapply enum_gmap_range_bounded'_spec; split=>//. *)
+    (*   intros ρ' tid' Hsome. unfold tids_smaller in *. *)
+    (*   apply locales_of_list_from_locale_from. eauto. } *)
+    (* rewrite elem_of_list_singleton; f_equal. *)
+    (* - destruct δ2; simpl. f_equal; apply ProofIrrelevance. *)
+    (* - destruct ℓ; simpl; destruct oζ =>//; by inversion Hlab. *)
+    (*   Unshelve. *)
+    (*   + intros ??. apply make_decision. *)
+    (*   + intros. apply make_proof_irrel. *)
+    (*   + done. *)
+    (*   + done. *)
+  Admitted.
 End finitary.
+
+
+Section finitary_simple.
+  Context `{M: FairModel}.
+  Context `{Λ: language}.
+  Context `{LM: LiveModel Λ M}.
+  Context `{EqDecision M}.
+  Context `{EqDecision (locale Λ)}.
+
+  Context `{HPI0: forall s x, ProofIrrel ((let '(s', ℓ) := x in M.(fmtrans) s ℓ s'): Prop) }.
+
+  Variable model_finitary: forall s1, Finite { '(s2, ℓ) | M.(fmtrans) s1 ℓ s2 }.
+
+  Lemma valid_state_evolution_finitary_fairness_simple (φ: execution_trace Λ -> auxiliary_trace LM -> Prop) :
+    rel_finitary (valid_lift_fairness φ).
+  Proof. Admitted.
+End finitary_simple.
